\documentclass[../../main.tex]{subfiles}

\begin{document}
\subsection{Theorem 1.1}

\begin{wts}
    $A\cap(B\cup C) = (A\cap B)\cup (A\cap C)$. 
\end{wts}

\begin{proof}
    We can use a chain of equivalences. Suppose that both members are not empty.
\begin{align*}
    x\in A\cap (B\cup C) &\iff x\in A\wedge x\in (B\cup C)\\
    &\iff x\in A \text{ and } (x\in B \text{ or }x\in C)\\
    &\iff (x\in A\wedge x\in B)\text{ or }(x\in A\wedge x\in C)\\
    &\iff x\in (A\cap B)\cup (A\cap C)
\end{align*}
Now suppose one of the two members are empty. Then if the other member was not empty, 
it would imply that the original member was not empty, and this means that the two sets must be equal.
\end{proof}
\end{document}