\documentclass[../../main.tex]{subfiles}

\begin{document}
\subsection{Theorem 1.2}
\begin{wts}
    $(A\setminus B)\cup(B\setminus A) = (A\cup B)\setminus(A\cap B)$.
\end{wts}

\begin{proof}
    Define $W = (A\setminus B)\cup (B\setminus A)$, then we will apply Q1a, and deMorgan's Theorem.
\begin{align*}
    W^c &= (A^c\cup B)\cap(B^c\cup A)\\
    &=((A^c\cup B)\cap B^c) \cup\, ((A^c\cup B)\cap A)\\
    &= (A^c \cap B^c)\cup (A\cap B)\\
    &= (A\cup B)^c \cup (A\cap B)\\
    &= [(A\cup B)\setminus(A\cap B)]^c
\end{align*}
Taking complements on both sides finishes the proof.
\end{proof}

\end{document}