\documentclass[../../main.tex]{subfiles}

\begin{document}
\subsection{Lemma}
\begin{lemma}\label{lemma:swap_sup_inf}
    If $A$ is a non-empty bounded above subset of $\mathbb{R}$, then $(-1)(\sup A) = \inf (-1)A$.
\end{lemma}
\begin{proof}
    Let $s=\sup(A)$, then
    \[
    (-1)A = \{-x: x\in A\}
    \]
    Evidently, for every $x\in A$
    \[
    x\leq s\implies -s\leq -x\implies -s\leq (-1)A
    \]
    Now fix any $\varepsilon>0$, then there exists an $x\in A$ such that
    \[
    s-\varepsilon\leq x\implies (-1)(s-\varepsilon)\geq -x\implies (-x)\leq (-s)+\varepsilon
    \]
    Thus establishes $\inf(-1)A=(-1)\sup(A)$.
\end{proof}
\begin{corollary}
    $(-1)\inf(A) = \sup(-1)A$. The proof is trivial just replace $A$ by $(-1)A$.
\end{corollary}
\end{document}